\input{settings} 
\begin{document}

\lhead{Yida Liu} 
\rhead{EECS 416 Spring 2020 \\ Convex Optimization for Engineering \\ Homework 8} 
\cfoot{\thepage\ of \pageref{LastPage}}

\section{Order and Rate of Convergence}

\subsection{$x^{(k)} = 2 + 0.2^k$}
\par Clearly, the algorithm converges to 2.
\[
\lim_{k \to \infty} \frac{||x^{k+1} - x^*||}{||x^{(k)} - x^*||} = \lim_{k \to \infty} \frac{ 0.2^{k + 1}}{0.2^{k}} = 0.2
\]
The algorithm converge at least linearly.
\[
\lim_{k \to \infty} \frac{||x^{(k+1)} - x^*||}{||x^{(k)} - x^*||^p} = \frac{0.2^{k+1}}{0.2^{kp}} = \frac{0.2}{0.2^{k(p - 1)}} = \infty
\]
Linear convergence.

\subsection{$x^{(k)} = 1 + (\frac{4}{k})^k$}
\begin{align*}
\lim_{k\to\infty} x^{(k)} = 1 + \lim_{k\to\infty} (\frac{4}{k})^k = 1
\end{align*}
\[
\lim_{x \to \infty} \frac{||x^{(k+1)} - x^*||}{||x^{(k)} - x^*||} = \frac{(4/(k+1))^{(k+1)}}{(4/k)^k} = 0
\]
The algorithm converge at least linearly.
\[
\lim_{k \to \infty} \frac{||x^{(k+1)} - x^*||}{||x^{(k)} - x^*||^p} = \frac{(4/(k+1))^{(k+1)}}{(4/k)^{pk}} = \infty
\]
Linear convergence.

\subsection{$x^{(k)} = 2^{-2^k}$}
\begin{align*}
\lim_{k\to\infty} x^{(k)} =  \lim_{k\to\infty} 2^{-2^k}= 0
\end{align*}
\[
\lim_{k \to \infty} \frac{||x^{(k+1)} - x^*||}{||x^{(k)} - x^*||} = \frac{2^{-2^{(k+1)}}}{2^{-2^k}} = 0
\]

The algorithm converge at least linearly.
\[
\lim_{k \to \infty} \frac{||x^{(k+1)} - x^*||}{||x^{(k)} - x^*||^p} = \frac{2^{-2^{(k+1)}}}{2^{-2^(pk)}} = \infty
\]
Linear convergence.

\subsection{$x^{(k+1)} = \frac{1}{2}x^{(k)} + \frac{8}{x^{(k)}}$}
Suppose the algorithm converges, we have
\[
x^* = \frac{1}{2}x^* + \frac{8}{x^{*}}
\]
\[
x^* = \pm 4
\]
The problem gives $x^{(0)} \leq 0$, we have $x^* = -4$.

\[
\lim_{k \to \infty} \frac{||x^{(k+1)} - x^*||}{||x^{(k)} - x^*||^2} = 
\lim_{k \to \infty} \frac{||\frac{1}{2}x^{(k)} + \frac{8}{x^{(k)}} + 4||}{||x^{(k)} + 4||^2} = \lim_{k \to \infty} \frac{1}{||2x^{(k)}||} = \frac{1}{8}
\]
The algorithm converges at order 2.

\section{Convergence of SD}

\[
f(\bm x) = x_1^2 + 2x_2^2
\]
Starting at $\bm x^{(0)} =\begin{pmatrix}2 \\ 1\end{pmatrix}$
\subsection{Recurrence Relation}
We verify that using numeric example for the first 5 iterations.
\begin{gather*}
x^{(1-5)} = \left(\begin{array}{ccccc}
2 & 0.6667 & 0.2222 & 0.0741 & 0.0247\\
1 & -0.3333 & 0.1111 & -0.0370 & 0.0123
\end{array}\right) \\
x_k^{(1-5)} = \left(\begin{array}{ccccc}
2 & 0.6667 & 0.2222 & 0.0741 & 0.0247\\
1 & -0.3333 & 0.1111 & -0.0370 & 0.0123
\end{array}\right)
\end{gather*}
which are equivalent. Similarly, 
\begin{gather*}
f^{(1-4)} / 9 = \left(\begin{array}{cccc}
0.6667 & 0.0741 & 0.0082 & \text{9.1111e-04}
\end{array}\right)\\
f^{(2-5)} = \left(\begin{array}{cccc}
0.6667 & 0.0741 & 0.0082 & \text{9.1449e-04}
\end{array}\right)
\end{gather*}
They are roughly equal. The error probably coming from round-off for division during the numeric computation.
\par \textit{See attached code for the validation of first 100 iteration. }

\subsection{$\bm x^*$ and Convergence Ratio}

\begin{align*}
\lim_{k\to\infty} x^{(k)} = \lim_{k\to\infty} \frac{1}{3^k}\begin{pmatrix}2 \\ (-1)^k\end{pmatrix} = \begin{pmatrix}0 \\ 0\end{pmatrix}
\end{align*}

\begingroup
\renewcommand*{\arraystretch}{1.6}
\[
\lim_{x \to \infty} \frac{||x^{(k+1)} - x^*||}{||x^{(k)} - x^*||} = \lim_{x \to \infty}
\frac
{\Bigg|\Bigg|\begin{pmatrix}
\frac{2}{3^{k+1}}\\
\frac{-1^{k+1}}{3^{k+1}}
\end{pmatrix}\Bigg|\Bigg|}
{\Bigg|\Bigg|\begin{pmatrix}
\frac{2}{3^{k}}\\
\frac{-1^{k}}{3^{k}}
\end{pmatrix}\Bigg|\Bigg|}
 = \frac{1}{3}
\]
\endgroup




\section{SD / NR}
\[
f(\bm x) = x_2 (x_1 -2) ^2 + 10(x_2 - 1)^2
\]
with $x^{(0)} = \begin{pmatrix}1 \\ 1\end{pmatrix}$. 

\subsection{SD}
\begin{itemize}
\item $k = 1$ \par 
\begin{gather*}
d = \begin{pmatrix} 2 \\ -1\end{pmatrix}\\
x^{(1)} = \left(\begin{array}{c}
2\,\alpha +1\\
1-\alpha 
\end{array}\right)\\
\phi = 10\,\alpha^2 -{{\left(2\,\alpha -1\right)}}^2 \,{\left(\alpha -1\right)} \\
\end{gather*}
Solve for optimal $\alpha$ 
\begin{gather*}
\alpha = 0.1460 \\
x^{(1)} = \left(\begin{array}{c}
1.2920\\
0.8540
\end{array}\right)
\end{gather*}
\item $k = 2$
\begin{gather*}
d = \left(\begin{array}{c}
1.2093\\
2.4186
\end{array}\right)\\
x^{(2)} = \left(\begin{array}{c}
1.2093\,\alpha +1.2920\\
2.4186\,\alpha +0.8540
\end{array}\right)\\
\phi = 10\,{{\left(2.4186\,\alpha -0.1460\right)}}^2 +{{\left(1.2093\,\alpha -0.7080\right)}}^2 \,{\left(2.4186\,\alpha +0.8540\right)}
\end{gather*}
Solve for optimal $\alpha$
\begin{gather*}
\alpha = 0.0653 \\
x^{(2)} = \left(\begin{array}{c}
1.3710\\
1.0120
\end{array}\right)
\end{gather*}
\end{itemize}

\subsection{NR}

\begin{enumerate}
\item $k = 1$
\begin{gather*}
H_f = \left(\begin{array}{cc}
2 & -2\\
-2 & 20
\end{array}\right)\\
g = \left(\begin{array}{c}
-2\\
1
\end{array}\right)\\
d = \left(\begin{array}{c}
1.0556\\
0.0556
\end{array}\right)ca \\
x^{(1)} = \left(\begin{array}{c}
1.0556\,\alpha +1\\
0.0556\,\alpha +1
\end{array}\right)\\
\phi = {{\left(1.0556\,\alpha -1\right)}}^2 \,{\left(0.0556\,\alpha +1\right)}+0.0309\,\alpha^2\\
\alpha = 0.9230\\
x^{(1)} =\left(\begin{array}{c}
1.9743\\
1.0513
\end{array}\right)
\end{gather*}

\item $k = 2$
\begin{gather*}
H_f = \left(\begin{array}{cc}
2.1026 & -0.0514\\
-0.0514 & 20
\end{array}\right)\\
g = \left(\begin{array}{c}
-0.0540\\
1.0263
\end{array}\right)\\
d = \left(\begin{array}{c}
0.0244\\
-0.0512
\end{array}\right)
x^{(2)} = \left(\begin{array}{c}
0.0244\,\alpha +1.9743\\
1.0513-0.0512\,\alpha 
\end{array}\right)\\
\phi =10\,{{\left(0.0512\,\alpha -0.0513\right)}}^2 -{\left(0.0512\,\alpha -1.0513\right)}\,{{\left(0.0244\,\alpha -0.0257\right)}}^2\\
\alpha = 1.0017 \\
x^{(2)} = \left(\begin{array}{c}
1.9988\\
0.9999
\end{array}\right)
\end{gather*}
\end{enumerate}

\end{document}